prove wp_shardOf_bound; start with wp_bytesEqual

src/program_proof/memkv/common_proof.v
@@ -5,9 +5,9 @@ Section common_proof.
 
 Context `{!heapG Σ}.
 
-Definition shardOfC (key:u64) : u64 := (word.modu key (65536%Z)).
-
 Definition uNSHARD : Z := 65536%Z.
+
+Definition shardOfC (key:u64) : u64 := (word.modu key uNSHARD).
 
 Lemma wp_shardOf key :
   {{{
@@ -33,13 +33,39 @@ Lemma wp_shardOf_bound (key:u64) :
      (s:u64), RET #s; ⌜int.Z s < uNSHARD⌝
   }}}.
 Proof.
-Admitted.
+  iIntros (Φ) "_ HΦ".
+  iApply wp_shardOf; first done.
+  iIntros "!> _". iApply "HΦ".
+  rewrite /shardOfC /uNSHARD.
+  iPureIntro. rewrite word.unsigned_modu_nowrap //.
+  apply Z.mod_pos_bound. done.
+Qed.
 
 Lemma wp_bytesEqual (x y : Slice.t) (xs ys : list byte) qx qy :
   {{{ typed_slice.is_slice x byteT qx xs ∗ typed_slice.is_slice y byteT qy ys }}}
     bytesEqual (slice_val x) (slice_val y)
   {{{ RET #(bool_decide (xs = ys)); typed_slice.is_slice x byteT qx xs ∗ typed_slice.is_slice y byteT qy ys }}}.
 Proof.
+  iIntros (Φ) "[Hx Hy] HΦ". wp_lam. wp_pures.
+  do 2 wp_apply wp_slice_len.
+  wp_pures.
+  iDestruct (typed_slice.is_slice_sz with "Hx") as %Hxlen.
+  iDestruct (typed_slice.is_slice_sz with "Hy") as %Hylen.
+  destruct_decide (bool_decide_reflect (#x.(Slice.sz) = #y.(Slice.sz))) as Hlen; last first.
+  { (* Different lengths. *)
+    wp_pures.
+    case_bool_decide as Hsl.
+    - subst ys. exfalso. apply Hlen. do 2 f_equal.
+      rewrite Hxlen in Hylen.
+      apply Z2Nat.inj in Hylen; [|word..].
+      apply (inj (R:=(=))) in Hylen; last by apply _.
+      done.
+    - iApply "HΦ". eauto with iFrame. }
+  wp_pures.
+  wp_apply wp_ref_to; first by val_ty.
+  iIntros (l) "Hi". wp_pures.
+  wp_apply wp_ref_to; first by val_ty.
+  iIntros (ret) "Hret". wp_pures.
 Admitted.
 
 End common_proof.
